Splinter/Paged/Bundle.i.dfy
@@ -1,0 +1,5 @@
+include "AbstractJournal.i.dfy"
+
+// Hey look, this abstract journal satisfies the refinement.
+module AbstractJournalRefinement refines PagedSystemRefinement(AbstractJournal) {
+}
