Splinter/Paged/JournalIfc.i.dfy
@@ -1,0 +1,83 @@
+// Copyright 2018-2021 VMware, Inc., Microsoft Inc., Carnegie Mellon University, ETH Zurich, and University of Washington
+// SPDX-License-Identifier: BSD-2-Clause
+
+include "../CoordinationLayer/MsgHistory.i.dfy"
+
+abstract module JournalIfc {
+  import opened Options
+  import opened MsgHistoryMod
+  import opened StampedMapMod // LSN TODO(jonh): move
+
+  // TODO(jonh): Recover and document why these are different types.
+  type PersistentJournal(==,!new)
+  type EphemeralJournal(==,!new)
+
+  predicate PWF(pj: PersistentJournal)
+  predicate EWF(ej: EphemeralJournal)
+
+  // Interpretations of these journals, for proof semantics (Refinement file).
+  function IPJ(pj: PersistentJournal) : (out:MsgHistory)
+    requires PWF(pj)
+    ensures out.WF()
+
+  function IEJ(ej: EphemeralJournal) : (out:MsgHistory)
+    requires EWF(ej)
+    ensures out.WF()
+
+  // Functions used in the runtime specification (this file).
+
+  function Mkfs() : (out:PersistentJournal)
+    ensures PWF(out)
+    ensures IPJ(out).EmptyHistory?
+
+  function LoadJournal(pj: PersistentJournal) : (out:EphemeralJournal)
+    requires PWF(pj)
+    ensures EWF(out)
+    ensures IEJ(out) == IPJ(pj)
+
+  // TODO rename PJournalSeqEnd, I guess
+  function JournalSeqEnd(pj: PersistentJournal) : (out:Option<LSN>)
+    requires PWF(pj)
+    ensures out.Some? == IPJ(pj).MsgHistory?
+    ensures out.Some? ==> out.value == IPJ(pj).seqEnd
+
+  function EJournalSeqEnd(ej: EphemeralJournal) : (out:Option<LSN>)
+    requires EWF(ej)
+    ensures out.Some? == IEJ(ej).MsgHistory?
+    ensures out.Some? ==> out.value == IEJ(ej).seqEnd
+
+  predicate JournalIncludesSubseq(ej: EphemeralJournal, msgs: MsgHistory)
+    requires EWF(ej)
+    requires msgs.WF()
+    ensures JournalIncludesSubseq(ej, msgs) <==> IEJ(ej).IncludesSubseq(msgs)
+
+  function JournalConcat(ej: EphemeralJournal, msgs: MsgHistory) : (out:EphemeralJournal)
+    requires EWF(ej)
+    requires msgs.WF()
+    requires msgs.EmptyHistory? || EJournalSeqEnd(ej).None? || msgs.CanFollow(EJournalSeqEnd(ej).value)
+    ensures EWF(JournalConcat(ej, msgs))
+    ensures EWF(out)
+    ensures IEJ(ej).Concat(msgs) == IEJ(out)
+
+  predicate JournalCanFreeze(ej: EphemeralJournal, startLsn: LSN, endLsn: LSN)
+    requires EWF(ej)
+    ensures JournalCanFreeze(ej, startLsn, endLsn) <==>
+      (IEJ(ej).CanDiscardTo(startLsn) && IEJ(ej).CanDiscardTo(endLsn))
+
+  function JournalFreeze(ej: EphemeralJournal, startLsn: LSN, endLsn: LSN) : (out:PersistentJournal)
+    requires EWF(ej)
+    requires JournalCanFreeze(ej, startLsn, endLsn)
+    requires startLsn <= endLsn
+    ensures PWF(out)
+    ensures IPJ(out) == IEJ(ej).DiscardOld(startLsn).DiscardRecent(endLsn)
+
+  predicate CanDiscardOld(ej: EphemeralJournal, lsn: LSN)
+    requires EWF(ej)
+    ensures CanDiscardOld(ej, lsn) <==> IEJ(ej).CanDiscardTo(lsn)
+
+  function DiscardOld(ej: EphemeralJournal, lsn: LSN) : (out:EphemeralJournal)
+    requires EWF(ej)
+    requires CanDiscardOld(ej, lsn)
+    ensures EWF(out)
+    ensures IEJ(out) == IEJ(ej).DiscardOld(lsn)
+}
